Compiler of typ instead dtyp

src/coq/Compiler/Compiler.v
@@ -46,11 +46,31 @@ Section Allocations.
 End Allocations.
 
 
+Fixpoint compile_decs_s (ds:list dec) :=
+match ds with
+  | nil => nil
+  | h :: t => match h with | Var x => [(LLVMAst.IId (LLVMAst.Name x), LLVMAst.INSTR_Alloca (TYPE_I 32) None None) ; (IVoid 0%Z, (INSTR_Store false ((TYPE_I 32%N), (EXP_Integer (Int32.unsigned (Int32.repr 0%Z)))) (TYPE_Pointer (TYPE_I 32), (EXP_Ident (ID_Local (Name x)))) None)) ] ++ (compile_decs_s t) end
+end.
+
 Fixpoint compile_decs (ds:list dec) :=
 match ds with
   | nil => nil
-  | h :: t => match h with | Var x => [(LLVMAst.IId (LLVMAst.Name x), LLVMAst.INSTR_Alloca (DynamicTypes.DTYPE_I 32) None None) ; (IVoid 0%Z, (INSTR_Store false ((DTYPE_I 32%N), (EXP_Integer (Int32.unsigned (Int32.repr 0%Z)))) (DTYPE_Pointer, (EXP_Ident (ID_Local (Name x)))) None)) ] ++ (compile_decs t) end
+  | h :: t => match h with | Var x => [(LLVMAst.IId (LLVMAst.Name x), LLVMAst.INSTR_Alloca (DTYPE_I 32) None None) ; (IVoid 0%Z, (INSTR_Store false ((DTYPE_I 32%N), (EXP_Integer (Int32.unsigned (Int32.repr 0%Z)))) (DTYPE_Pointer, (EXP_Ident (ID_Local (Name x)))) None)) ] ++ (compile_decs t) end
 end.
+
+Definition compile_stmt_s (s : stmt) : code typ :=
+  match s with
+  | Skip => nil
+  | Assign x v => match v with 
+                  | Lit n => [(IVoid 0%Z, (INSTR_Store false ((TYPE_I 32%N), (EXP_Integer (Int32.unsigned n))) (TYPE_Pointer (TYPE_I 32), (EXP_Ident (ID_Local (Name x)))) None))]
+                  end
+  end.
+
+Fixpoint compile_stmts_s (ss : list stmt) : code typ :=
+  match ss with
+  | nil => []
+  | h :: t => (compile_stmt_s h) ++ (compile_stmts_s t)
+  end.
 
 Definition compile_stmt (s : stmt) : code dtyp :=
   match s with
@@ -66,10 +86,126 @@ Fixpoint compile_stmts (ss : list stmt) : code dtyp :=
   | h :: t => (compile_stmt h) ++ (compile_stmts t)
   end.
 
-Definition compile (p : AST.prog) : code dtyp :=
+
+Definition compile (p : AST.prog) : code typ :=
   match p with
-  | Prog ds ss => (compile_decs ds) ++ (compile_stmts ss)
+  | Prog ds ss => (compile_decs_s ds) ++ (compile_stmts_s ss)
   end.
+
+(* Lemma convert_typ_code_cons: forall a (b : code typ) env, (convert_typ env (a :: b) = convert_typ env a ++ convert_typ env b)%list.
+Proof.
+  induction a as [| [] a IH]; cbn; intros; auto.
+  rewrite IH; reflexivity.
+Qed.
+ *)
+
+Lemma cons_app_singleton : forall (A : Type) (h : A) (t : list A),
+  h :: t = [h] ++ t.
+Proof.
+  reflexivity.
+Qed.
+
+
+Lemma compile_decs_cons_app_singleton : forall t h,
+compile_decs (h :: t) = compile_decs [h] ++ compile_decs t.
+Proof.
+intros.
+unfold compile_decs.
+destruct h.
+reflexivity.
+Qed.
+
+Lemma compile_decs_s_cons_app_singleton : forall t h,
+compile_decs_s (h :: t) = compile_decs_s [h] ++ compile_decs_s t.
+Proof.
+intros.
+unfold compile_decs_s.
+destruct h.
+reflexivity.
+Qed.
+
+Lemma convert_typ_decs_singleton : forall a,
+convert_typ [] (compile_decs_s [a]) = compile_decs [a].
+Proof.
+intros.
+destruct a.
+unfold convert_typ.
+cbn.
+repeat rewrite TypToDtyp.typ_to_dtyp_equation.
+reflexivity.
+Qed.
+
+Lemma convert_typ_decs: forall ds,
+TypToDtyp.convert_typ [] (compile_decs_s ds) = (compile_decs ds).
+Proof.
+induction ds.
++ simpl.
+  unfold convert_typ.
+  auto.
++ rewrite compile_decs_s_cons_app_singleton.
+  symmetry.
+  rewrite compile_decs_cons_app_singleton.
+  rewrite TypToDtyp.convert_typ_code_app.
+  rewrite convert_typ_decs_singleton.
+  rewrite IHds.
+  reflexivity.
+Qed.
+
+
+Lemma compile_stmts_cons_app_singleton : forall t h,
+compile_stmts (h :: t) = compile_stmts [h] ++ compile_stmts t.
+Proof.
+intros.
+unfold compile_stmts.
+destruct h; simpl.
++ destruct e.
+  reflexivity.
++ reflexivity.
+Qed.
+
+Lemma compile_stmts_s_cons_app_singleton : forall t h,
+compile_stmts_s (h :: t) = compile_stmts_s [h] ++ compile_stmts_s t.
+Proof.
+intros.
+unfold compile_stmts_s.
+destruct h; simpl.
++ destruct e.
+  reflexivity.
++ reflexivity.
+Qed.
+
+Lemma convert_typ_stmts_singleton : forall a,
+convert_typ [] (compile_stmts_s [a]) = compile_stmts [a].
+Proof.
+intros.
+destruct a.
++ simpl.
+  destruct e.
+  unfold convert_typ.
+  cbn.
+  repeat rewrite TypToDtyp.typ_to_dtyp_equation.
+  reflexivity.
++ simpl.
+  unfold convert_typ.
+  cbn.
+  reflexivity.
+Qed.
+
+Lemma convert_typ_stmts: forall ds,
+TypToDtyp.convert_typ [] (compile_stmts_s ds) = (compile_stmts ds).
+Proof.
+induction ds.
++ simpl.
+  unfold convert_typ.
+  auto.
++ rewrite compile_stmts_s_cons_app_singleton.
+  symmetry.
+  rewrite compile_stmts_cons_app_singleton.
+  rewrite TypToDtyp.convert_typ_code_app.
+  rewrite convert_typ_stmts_singleton.
+  rewrite IHds.
+  reflexivity.
+Qed.
 
 
 
